add attempts to prove complete behavior preservation

LTT_PLTT.v
@@ -6,6 +6,8 @@ Require Import PLTT.
 Require Import Smallstep.
 Require Import Behavior.
 
+Require Import Coq.Logic.Classical.
+
 Module LTT_TO_PLTT.
 
 Include AbstractMachine.
@@ -354,51 +356,291 @@ Section SIMULATION.
     apply forward_simulation_between_LTT_and_PLTT.
   Qed.
 
-  Theorem wrong_behavior_preservation:
-    forall t,
-      program_behaves (LTT.semantics p) (Goes_wrong t) ->
-      program_behaves (PLTT.semantics pp) (Goes_wrong t).
+  (* END OF STABLE PART *)
+
+  (* We can prove something stronger, that is, PLTT 
+     preserves exactly all behaviors. *)
+
+  (* IDEA:
+     when LTT goes wrong we might be in two cases:
+     - the program is executing
+       it means that PLTT must be stuck as well
+     - the context is executing
+       it means that the last step of our simulation
+       must go into a WentWrong state
+     by proving this two lemmas, we should be able to
+     show that the trace produced when going wrong
+     is exactly the same.
+   *)
+
+  Lemma nonfinal_preservation_for_program:
+    forall s pstate,
+      match_states split s (PLTT.PC pstate) ->
+      ~ LTT.final_state s ->
+      ~ PLTT.final_state (PLTT.PC pstate).
   Proof.
-    intros t Hprogbeh.
-    destruct forward_simulation_between_LTT_and_PLTT
-      as [index order generic_match_states S].
-    remember S as sim_prop.
-    destruct S as [? Hmatch_initial Hmatch_final Hsim].
-    inversion Hprogbeh.
-    - destruct (Hmatch_initial s) as [i]; auto.
-      destruct H2 as [ps [Hps_init Hps_match]].
-      apply program_runs with ps.
-      + auto.
-      + inversion H0.
-        destruct (simulation_star sim_prop H3 i ps Hps_match)
-          as [i' [ps' [Hps_star Hps'_match]]].
-        apply state_goes_wrong with ps'; auto.
-    (* stuck! I can't reason on our specific instance 
-       of match_states, hence I cannot demonstrate that 
-       PLTT cannot step! *)
+    intros s pstate Hmatch_states Hnot_final.
+    unfold not, PLTT.final_state.
+    destruct pstate. destruct p0. destruct p0. destruct p0.
+    intro Hhalt.
+    apply Hnot_final. unfold LTT.final_state.
+    destruct s. destruct p0. destruct p0. destruct p0.
+    inversion Hmatch_states; subst. auto.
+  Qed.
+
+  Lemma nostep_preservation_for_program:
+    forall s pstate,
+      match_states split s (PLTT.PC pstate) ->
+      (forall t s', ~ LTT.step G s t s') -> 
+      (forall t ps', ~ PLTT.step G' (PLTT.PC pstate) t ps'). 
+  Proof.
+    intros s pstate Hmatch_states Hnostep.
+    intros t ps'. unfold not. intro contra.
+    inversion Hmatch_states. subst.
+    inversion contra; subst.
+    apply Hnostep with (t:=E0) (s':=(C,s0,mem',regs,pc')).
+    (* apply LTT weakening *)
+    Admitted.
+
+  (* 1st ATTEMPT *)
+  
+  Section FORWARD_SIMULATION.
+    Context index order match_states
+            (S: fsim_properties
+                  (LTT.semantics p) (PLTT.semantics pp)
+                  index order match_states).
+
+    Lemma generic_match_implies_specific_match:
+      forall i s pstate,
+        match_states i s (PLTT.PC pstate) ->
+        SIMULATION.match_states split s (PLTT.PC pstate).
+    Proof.
+      intros i s pstate Hmatch_states.
+    Admitted.
+
+    Lemma goes_wrong_preservation:
+      forall i s ps t s',
+        Star (LTT.semantics p) s t s' ->
+        Nostep (LTT.semantics p) s' ->
+        ~final_state (LTT.semantics p) s' ->
+        match_states i s ps ->
+      exists ps',
+        Star (PLTT.semantics pp) ps t ps' /\
+        Nostep (PLTT.semantics pp) ps' /\
+        ~final_state (PLTT.semantics pp) ps'.
+    Proof.
+      intros i s ps t s'.
+      intros HLTT_star HLTT_nostep HLTT_nofinal.
+      intros Hmatch_states.
+      destruct (simulation_star
+                  S HLTT_star i ps Hmatch_states)
+        as [i' [ps' [HPLTT_star Hmatch_states']]].
+      destruct ps' as [pstate | cstate exec_state].
+      (* the program got stuck *)
+      - exists (PLTT.PC pstate). split; auto. split.
+        (* we cannot step anymore *)
+        + simpl. unfold nostep.
+          rewrite p_transfto_pp.
+          unfold PLTT.apply_split. simpl.
+          eapply nostep_preservation_for_program;
+            eauto.
+          apply (generic_match_implies_specific_match i');
+            auto.
+        (* we are not in a final state *)
+        + apply nonfinal_preservation_for_program with s';
+            eauto.
+          apply (generic_match_implies_specific_match i');
+            auto.
+      (* the context got stuck *)
+      - exists (PLTT.CC cstate PLTT.WentWrong).
+        split.
+        * destruct exec_state.
+          ** apply star_right with
+                 t (PLTT.CC cstate PLTT.Normal) E0.
+             *** apply HPLTT_star.
+             *** destruct cstate. destruct p0.
+                 apply PLTT.Context_GoesWrong.
+             *** symmetry. apply E0_right.
+          ** auto.
+        * split.
+          (* WentWrong doesn't step *)
+          ** unfold nostep. intros.
+             unfold not. intro contra. inversion contra.
+          (* WentWrong is not final *)
+          ** unfold not. intro.
+             enough (Hnot_final:
+                       ~ PLTT.final_state
+                         (PLTT.CC cstate PLTT.WentWrong)).
+             apply Hnot_final; auto.
+             unfold not, PLTT.final_state.
+             destruct cstate. destruct p0.
+             intro contra. inversion contra.
+    Qed.
+
+    Theorem state_goes_wrong_preservation:
+      forall i s ps t,
+        match_states i s ps ->
+        state_behaves (LTT.semantics p) s (Goes_wrong t) ->
+        state_behaves (PLTT.semantics pp) ps (Goes_wrong t).
+    Proof.
+      intros i s ps t Hmatch_states Hstatebeh.
+      inversion Hstatebeh.
+      destruct (goes_wrong_preservation
+             i s ps t s' H0 H1 H2 Hmatch_states)
+        as [ps' [Hps_star [Hps_nostep Hps_notfinal]]].
+      eapply state_goes_wrong; eauto.
+    Qed.
+
+    Theorem wrong_behavior_preservation:
+      forall t,
+        program_behaves (LTT.semantics p) (Goes_wrong t) ->
+        program_behaves (PLTT.semantics pp) (Goes_wrong t).
+    Proof.
+      intros t Hprogbeh.
+      inversion Hprogbeh as [ s beh Hs_init Hstatebeh
+                            | Hnot_init ].
+      (* goes wrong with non-empty trace *)
+      - (* initial states *)
+        destruct (fsim_match_initial_states S s Hs_init)
+          as [i [ps [Hps_init Hmatch_states]]].
+        (* simulation *)
+        eapply program_runs; eauto.
+        apply state_goes_wrong_preservation with i s; auto.
+      (* goes intially wrong *)
+      - assert (Hgoingwrong_state:
+          exists ps,
+            ps = (PLTT.CC (0%nat, [],
+                           @M.empty (list nat))
+                          PLTT.WentWrong) /\
+            Nostep (PLTT.semantics pp) ps /\
+            PLTT.initial_state pp ps /\
+            ~PLTT.final_state ps). {
+          exists (PLTT.CC (0%nat, [], @M.empty (list nat))
+                          PLTT.WentWrong).
+          split; auto.
+          split.
+          - unfold nostep. intros.
+            unfold not. intro contra. inversion contra.
+          - unfold PLTT.initial_state. split; auto.
+            unfold PLTT.final_state.
+            unfold not. intro contra. inversion contra.
+        }
+        destruct Hgoingwrong_state
+          as [ps [Hps_state [Hps_nostep
+                               [Hps_init Hps_notfinal]]]].
+        apply program_runs with ps; eauto. subst.
+        apply state_goes_wrong with
+            (PLTT.CC (0%nat, [], M.empty (list nat))
+                     PLTT.WentWrong).
+        apply star_refl; auto.
+        unfold nostep. intros t ps' contra.
+        inversion contra.
+        unfold not. intro contra.
+        apply Hps_notfinal. auto.
+    Qed.
+  End FORWARD_SIMULATION.
+
+  Corollary strong_behavior_preservation:
+    forall beh,
+      program_behaves (LTT.semantics p) beh ->
+      program_behaves (PLTT.semantics pp) beh.
+  Proof.
+    intros beh Hprogbeh.
+    destruct beh.
+    - eapply forward_simulation_same_safe_behavior; eauto.
+      apply forward_simulation_between_LTT_and_PLTT.
+      simpl. reflexivity.
+    - eapply forward_simulation_same_safe_behavior; eauto.
+      apply forward_simulation_between_LTT_and_PLTT.
+      simpl. reflexivity.
+    - eapply forward_simulation_same_safe_behavior; eauto.
+      apply forward_simulation_between_LTT_and_PLTT.
+      simpl. reflexivity.
+    - destruct forward_simulation_between_LTT_and_PLTT.
+      apply wrong_behavior_preservation with
+          index order match_states0; auto.
+  Qed.
+
+  (* STUCK! We cannot prove the two lemmas about
+     generic nostep and nonfinal preservation! *)
+
+  (* 2nd ATTEMPT *)
+  (* Let's try with a stronger notion of simulation *)
+
+  Record fsim_properties'
+         (L1 L2: semantics) (index: Type)
+         (order: index -> index -> Prop)
+         (match_states: index -> state L1 -> state L2 -> Prop)
+    : Prop := {
+      fsim_order_wf': well_founded order;
+      fsim_match_initial_states':
+        forall s1, initial_state L1 s1 ->
+        exists i, exists s2,
+            initial_state L2 s2 /\ match_states i s1 s2;
+      fsim_match_final_states':
+        forall i s1 s2,
+          match_states i s1 s2 ->
+          final_state L1 s1 -> final_state L2 s2;
+      fsim_simulation':
+        forall s1 t s1', Step L1 s1 t s1' ->
+        forall i s2, match_states i s1 s2 ->
+        exists i', exists s2',
+          (Plus L2 s2 t s2' \/
+           (Star L2 s2 t s2' /\ order i' i)) /\
+          match_states i' s1' s2';
+      fsim_match_stuck_states:
+        forall i s1 s2,
+          match_states i s1 s2 ->
+          Nostep L1 s1 ->
+          Nostep L2 s2;
+      fsim_match_nonfinal_states:
+        forall i s1 s2,
+          match_states i s1 s2 ->
+          ~ (final_state L1 s1) ->
+          ~ (final_state L2 s2)
+  }.
+
+  Arguments fsim_properties': clear implicits.
+
+  Inductive forward_simulation' (L1 L2: semantics) : Prop :=
+    Forward_simulation' (index: Type)
+                       (order: index -> index -> Prop)
+                       (match_states: index -> state L1 -> state L2 -> Prop)
+                       (props: fsim_properties' L1 L2 index order match_states).
+
+  Arguments Forward_simulation' {L1 L2 index} order match_states props.
+  
+  Lemma stronger_forward_LTT_PLTT:
+    forward_simulation' (LTT.semantics p) (PLTT.semantics pp).
+  Proof.
+    destruct forward_simulation_between_LTT_and_PLTT.
+    destruct props.
+    econstructor.
+    constructor; eauto.
+    (* stuck states *)
+    - admit.
+    (* non final states *)
+    - admit.
   Admitted.
 
   Require Import Coqlib.
-  
-  Lemma nostep_aux:
-    forall s ps,
-      match_states split s ps ->
-      (forall s' t, ~ (LTT.step G s t s')) ->
-      (forall ps' t, ~ (PLTT.step G' ps t ps')).
-  Proof.
-    intros s ps Hmatch_states Hnostep.
-    destruct s
-      as [[[[C d] mem] regs] pc] eqn:Hstate_s.
-    inversion Hmatch_states; subst; intros.
-    - admit. (* feasible *)
-    - admit.
-    - intro contra. inversion contra.
-  Qed.
+  Require Import Classical.
 
-  Section FORWARD_SIMULATION.
+  Section FORWARD_SIMULATION_2.
     Context index order match_states
-            (S: fsim_properties (LTT.semantics p) (PLTT.semantics pp)
-                                index order match_states).
+            (S': fsim_properties'
+                   (LTT.semantics p) (PLTT.semantics pp)
+                   index order match_states).
+
+    Let S := {|
+              fsim_order_wf :=
+                fsim_order_wf' _ _ _ _ _ S';
+              fsim_match_initial_states :=
+                fsim_match_initial_states' _ _ _ _ _ S';
+              fsim_match_final_states :=
+                fsim_match_final_states' _ _ _ _ _ S';
+              fsim_simulation :=
+                fsim_simulation' _ _ _ _ _ S' |}.
 
     Lemma forward_simulation_state_behaves:
       forall i s1 s2 beh,
@@ -418,43 +660,55 @@ Section SIMULATION.
       - (* going wrong *)
         exploit simulation_star; eauto. intros [i' [s2' [A B]]].
         econstructor; eauto.
-        (* stuck!! *)
-    Admitted.
-  End FORWARD_SIMULATION.
+        + apply (fsim_match_stuck_states _ _ _ _ _ S')
+            with i' s'; eauto.
+        + apply (fsim_match_nonfinal_states _ _ _ _ _ S')
+            with i' s'; eauto.
+    Qed.
 
-  Theorem behavior_preservation':
-    forall beh,
-      program_behaves (LTT.semantics p) beh ->
-      program_behaves (PLTT.semantics pp) beh.
-  Proof.
-    intros beh Hprogbeh.
-    destruct (forward_simulation_behavior_improves
-                forward_simulation_between_LTT_and_PLTT
-                Hprogbeh) as [beh2 [Hprogbeh2 Hbehimp]].
-    destruct forward_simulation_between_LTT_and_PLTT
-      as [? ? generic_match_states S].
-    unfold behavior_improves in Hbehimp.
-    inversion Hbehimp.
-    - subst. auto.
-    - destruct H as [t [Hgoeswrong Hbehprefix]].
-      rewrite Hgoeswrong.
-      destruct Hprogbeh.
-      (* initial states *)
-      destruct (initial_states_match s H)
-          as [ps [Hps_init Hmatch_states]].
-      (* star simulation *)
-      inversion H0.
-      + subst. inversion H3.
-      + subst. inversion H3.
-      + subst. inversion H2.
-      + subst. inversion H4.
-        eapply program_runs.
-        * eauto.
-        * admit. (*eapply state_goes_wrong.
-          ** pose (simulation_star S H1).*)
-      + subst. inversion Hgoeswrong. subst.
-        apply program_goes_initially_wrong.
-        intros. unfold not. intro.
-  Admitted.
+    Theorem behavior_preservation:
+      forall beh,
+        program_behaves (LTT.semantics p) beh ->
+        program_behaves (PLTT.semantics pp) beh.
+    Proof.
+      destruct stronger_forward_LTT_PLTT as [init ? ?].
+      intros. inversion H.
+      - (* initial state defined *)
+        exploit (fsim_match_initial_states S); eauto.
+        intros [i [s' [INIT MATCH]]].
+        + econstructor; eauto.
+          eapply forward_simulation_state_behaves; eauto.
+      - (* initial state undefined *)
+        assert (Hgoingwrong_state:
+                  exists ps,
+                    ps = (PLTT.CC (0%nat, [],
+                                   @M.empty (list nat))
+                                  PLTT.WentWrong) /\
+                    Nostep (PLTT.semantics pp) ps /\
+                    PLTT.initial_state pp ps /\
+                    ~PLTT.final_state ps). {
+          exists (PLTT.CC (0%nat, [], @M.empty (list nat))
+                          PLTT.WentWrong).
+          split; auto.
+          split.
+          - unfold nostep. intros.
+            unfold not. intro contra. inversion contra.
+          - unfold PLTT.initial_state. split; auto.
+            unfold PLTT.final_state.
+            unfold not. intro contra. inversion contra.
+        }
+        destruct Hgoingwrong_state
+          as [ps [Hps_state [Hps_nostep [Hps_init Hps_notfinal]]]].
+        apply program_runs with ps; eauto.
+        subst.
+        apply state_goes_wrong
+          with (PLTT.CC (0%nat, [], M.empty (list nat))
+                        PLTT.WentWrong).
+        apply star_refl. auto.
+        unfold not. intro contra. apply Hps_notfinal.
+        auto.
+    Qed.
+  End FORWARD_SIMULATION_2.
+  (* Stuck! Even here we have problems with the same lemmas! *)
 End SIMULATION.
 End LTT_TO_PLTT.
